# Additional Exercise 6

## Show that $$a_{n} = 3  \cdot 2^{n} + 7 \cdot 5^{n}$$ is a solution to the recurrence relation $$a_{n} = 7a_{n-1} - 10a_{n-2}$$. What would the initial conditions need to be for this to be the closed formula for the sequence?

## First find some of the terms using the closed formula:

$$a_{0} = 3  \cdot 2^{0} + 7 \cdot 5^{0} = 10$$

$$a_1 = 3 \cdot 2^1 + 7 \cdot 5^1 = 41$$

$$a_2 = 3 \cdot 2^2 + 7 \cdot 5^2 = 187$$

$$a_3 = 3 \cdot 2^3 + 7 \cdot 5^3 = 899$$


## Then, you can check to see if they fit the recurrence relation

According to the relation: $$a_2 = 7a_1 - 10a_0 = 7 \cdot 41 - 10 \cdot 10 = 187$$, which matches the $$a_2$$ term from the closed formula

When calculating the rest of the terms, you get

$$a_2 = 7a_1 - 10a_0 = 187$$

$$a_3 = 7a_2 - 10a_1 = 899$$



## All of the terms from the reccurence relation match the terms from the closed formula, showing that $$a_{n} = 3  \cdot 2^{n} + 7 \cdot 5^{n}$$ is a solution to $$a_{n} = 7a_{n-1} - 10a_{n-2}$$
